move precomp_get to Hacl.Impl.PrecompTable

code/bignum/Hacl.Impl.PrecompTable.fst
@@ -243,3 +243,27 @@ let lprecomp_table #a_t len ctx_len k ctx a table_len table =
   Lib.Loops.for 0ul (table_len -! 1ul) inv
   (fun j ->
     lprecomp_table_f #a_t len ctx_len k ctx a table_len j table)
+
+
+let lprecomp_get_vartime #a_t len ctx_len k a table_len table bits_l tmp =
+  let bits_l32 = Lib.RawIntTypes.(size_from_UInt32 (u32_to_UInt32 (to_u32 bits_l))) in
+  assert (v bits_l32 == v bits_l /\ v bits_l < v table_len);
+  Math.Lemmas.lemma_mult_le_right (v len) (v bits_l + 1) (v table_len);
+  assert (v (bits_l32 *! len) == v bits_l32 * v len);
+
+  let h0 = ST.get () in
+  let a_bits_l = sub table (bits_l32 *! len) len in
+  let h1 = ST.get () in
+  assert (precomp_table_inv len ctx_len k (as_seq h0 a) table_len (as_seq h0 table) (v bits_l));
+  assert (k.to.refl (as_seq h1 a_bits_l) == SE.pow k.to.concr_ops (k.to.refl (as_seq h0 a)) (v bits_l));
+  copy tmp a_bits_l
+
+
+let lprecomp_get_consttime #a_t len ctx_len k a table_len table bits_l tmp =
+  Math.Lemmas.lemma_mult_le_right (v len) (v bits_l + 1) (v table_len);
+  let h0 = ST.get () in
+  table_select_consttime len table_len table bits_l tmp;
+  let h1 = ST.get () in
+  assert (as_seq h1 tmp == LSeq.sub (as_seq h0 table) (v bits_l * v len) (v len));
+  assert (precomp_table_inv len ctx_len k (as_seq h0 a) table_len (as_seq h0 table) (v bits_l));
+  assert (k.to.refl (as_seq h1 tmp) == SE.pow k.to.concr_ops (k.to.refl (as_seq h0 a)) (v bits_l))
